template-coq/theories/Weakening.v
@@ -1,182 +1,15 @@
 (* Distributed under the terms of the MIT license.   *)
 
-From Coq Require Import Bool String List Program BinPos Compare_dec Omega.
+From Coq Require Import Bool String List Program BinPos Compare_dec Omega Lia.
 From Template Require Import config utils Ast AstUtils Induction utils LiftSubst Typing.
+From Template Require Import WeakeningEnv Closed.
 
-(** * Weakening and substitution lemmas for typing derivations.
+(** * Weakening lemmas for typing derivations.
 
-  *WIP*
-
-  Standard structural lemmas on typing derivations. *)
+  [weakening_*] proves weakening of typing, reduction etc... w.r.t. the *local* environment. *)
 
 Set Asymmetric Patterns.
-
 Generalizable Variables Σ Γ t T.
-
-Definition extends (Σ Σ' : global_context) :=
-  exists Σ'', Σ' = (Σ'' ++ fst Σ, snd Σ)%list.
-
-Lemma lookup_env_Some_fresh `{checker_flags} Σ φ c decl :
-  wf (Σ, φ) -> lookup_env Σ c = Some decl ->
-  ~ (fresh_global c Σ).
-Proof. unfold wf. unfold on_global_env; simpl.
-  induction 1; simpl. congruence.
-  destruct ident_eq eqn:Heq. intros [= ->].
-  rewrite <- (reflect_iff _ _ (ident_eq_spec _ _)) in Heq.
-  intro. inv H0. congruence.
-  intros Hl; specialize (IHX Hl).
-  intro. inv H0. contradiction.
-Qed.
-
-Lemma extends_lookup `{checker_flags} Σ Σ' c decl :
-  wf Σ' -> extends Σ Σ' ->
-  lookup_env (fst Σ) c = Some decl -> lookup_env (fst Σ') c = Some decl.
-Proof.
-  intros wfΣ' [Σ'' ->]. simpl.
-  induction Σ'' in wfΣ', c, decl |- *. simpl. auto.
-  specialize (IHΣ'' c decl). forward IHΣ''.
-  inv wfΣ'. simpl in X0. apply X.
-  intros HΣ. specialize (IHΣ'' HΣ).
-  inv wfΣ'. simpl in *.
-  destruct (ident_eq c (global_decl_ident a)) eqn:Heq'.
-  eapply lookup_env_Some_fresh in IHΣ''; eauto.
-  rewrite <- (reflect_iff _ _ (ident_eq_spec _ _)) in Heq'.
-  rewrite <- Heq' in H0. contradiction.
-  auto.
-Qed.
-Hint Resolve extends_lookup : extends.
-
-Lemma extends_wf_local:
-  forall (H : checker_flags) (Σ : global_context) (Γ : context),
-    wf_local Σ Γ ->
-    All_local_env
-      (fun (Σ0 : global_context) (Γ0 : context) (t T : term) =>
-         forall Σ' : global_context, wf Σ' -> extends Σ0 Σ' -> Σ';;; Γ0 |- t : T) Σ Γ ->
-    forall Σ' : global_context, wf Σ' -> extends Σ Σ' -> wf_local Σ' Γ.
-Proof.
-  intros H Σ Γ X X0 Σ' H0.
-  induction X; inv X0; try econstructor; auto.
-Qed.
-Hint Resolve extends_wf_local : extends.
-
-Lemma weakening_env_red1 `{CF:checker_flags} Σ Σ' Γ M N :
-  wf Σ' -> extends Σ Σ' ->
-  red1 (fst Σ) Γ M N ->
-  red1 (fst Σ') Γ M N.
-Proof.
-  induction 3 using red1_ind_all; try econstructor; eauto.
-  eapply extends_lookup in H0; eauto.
-
-  induction H0; constructor; intuition eauto.
-  induction H0; constructor; intuition eauto.
-  induction H0; constructor; intuition eauto.
-Qed.
-
-Lemma weakening_env_cumul `{CF:checker_flags} Σ Σ' Γ M N :
-  wf Σ' -> extends Σ Σ' ->
-  cumul Σ Γ M N -> cumul Σ' Γ M N.
-Proof.
-  intros wfΣ [Σ'' ->].
-  induction 1; simpl.
-
-  econstructor; eauto.
-
-  econstructor 2; eauto. eapply weakening_env_red1; eauto. exists Σ''; eauto.
-  econstructor 3; eauto. eapply weakening_env_red1; eauto. exists Σ''; eauto.
-Qed.
-
-Lemma weakening_env_consistent_universe_context_instance:
-  forall (Σ : global_context) (u : list Level.t) univs,
-    consistent_universe_context_instance Σ univs u ->
-    forall Σ' : global_context,
-      extends Σ Σ' -> consistent_universe_context_instance Σ' univs u.
-Proof.
-  intros Σ u univs H1 Σ' H2. destruct univs; simpl in *; eauto.
-  destruct UContext.dest. destruct H2 as [Σ'' ->]. simpl. auto.
-Qed.
-Hint Resolve weakening_env_consistent_universe_context_instance : extends.
-
-Lemma weakening_env_declared_constant:
-  forall (H : checker_flags) (Σ : global_context) (cst : ident) (decl : constant_body),
-    declared_constant (fst Σ) cst decl ->
-    forall Σ' : global_context, wf Σ' -> extends Σ Σ' -> declared_constant (fst Σ') cst decl.
-Proof.
-  intros H Σ cst decl H0 Σ' X2 H2.
-  eapply extends_lookup; eauto.
-Qed.
-Hint Resolve weakening_env_declared_constant : extends.
-
-Lemma weakening_env_declared_minductive:
-  forall (H : checker_flags) (Σ : global_context) ind decl,
-    declared_minductive (fst Σ) ind decl ->
-    forall Σ' : global_context, wf Σ' -> extends Σ Σ' -> declared_minductive (fst Σ') ind decl.
-Proof.
-  intros H Σ cst decl H0 Σ' X2 H2.
-  eapply extends_lookup; eauto.
-Qed.
-Hint Resolve weakening_env_declared_minductive : extends.
-
-Lemma weakening_env_declared_inductive:
-  forall (H : checker_flags) (Σ : global_context) ind mdecl decl,
-    declared_inductive (fst Σ) ind mdecl decl ->
-    forall Σ' : global_context, wf Σ' -> extends Σ Σ' -> declared_inductive (fst Σ') ind mdecl decl.
-Proof.
-  intros H Σ cst decl H0 [Hmdecl Hidecl] Σ' X2 H2. split; eauto with extends.
-Qed.
-Hint Resolve weakening_env_declared_inductive : extends.
-
-Lemma weakening_env_declared_constructor :
-  forall (H : checker_flags) (Σ : global_context) ind mdecl idecl decl,
-    declared_constructor (fst Σ) ind mdecl idecl decl ->
-    forall Σ' : global_context, wf Σ' -> extends Σ Σ' ->
-    declared_constructor (fst Σ') ind mdecl idecl decl.
-Proof.
-  intros H Σ cst mdecl idecl cdecl [Hidecl Hcdecl] Σ' X2 H2.
-  split; eauto with extends.
-Qed.
-Hint Resolve weakening_env_declared_constructor : extends.
-
-Lemma weakening_env_declared_projection :
-  forall (H : checker_flags) (Σ : global_context) ind mdecl idecl decl,
-    declared_projection (fst Σ) ind mdecl idecl decl ->
-    forall Σ' : global_context, wf Σ' -> extends Σ Σ' ->
-    declared_projection (fst Σ') ind mdecl idecl decl.
-Proof.
-  intros H Σ cst mdecl idecl cdecl [Hidecl Hcdecl] Σ' X2 H2.
-  split; eauto with extends.
-Qed.
-Hint Resolve weakening_env_declared_projection : extends.
-
-Lemma weakening_All_local_env_impl `{checker_flags}
-      (P Q : global_context -> context -> term -> term -> Type) Σ Σ' l :
-  All_local_env P Σ l ->
-  (forall Γ t T, P Σ Γ t T -> Q Σ' Γ t T) ->
-  All_local_env Q Σ' l.
-Proof.
-  induction 1; intros; simpl; econstructor; eauto. Qed.
-
-Lemma weakening_env `{checker_flags} :
-  env_prop (fun Σ Γ t T =>
-              forall Σ', wf Σ' -> extends Σ Σ' -> Σ' ;;; Γ |- t : T).
-Proof.
-  apply typing_ind_env; intros; try solve [econstructor; eauto 2 with extends].
-
-  - econstructor; eauto.
-    clear H0 H1 X X0. induction X1 in wfΓ |- *; econstructor; eauto.
-    eapply weakening_env_cumul in cumul; eauto.
-  - econstructor; eauto 2 with extends.
-    destruct H6 as [Σ'' ->]. simpl; auto.
-    close_Forall. intros; intuition eauto with extends.
-  - econstructor; eauto with extends.
-    eapply weakening_All_local_env_impl. eapply X.
-    clear -X1 H0. simpl; intros. intuition eauto with extends.
-    eapply All_impl; eauto; simpl; intuition eauto with extends.
-  - econstructor; eauto with extends.
-    eapply weakening_All_local_env_impl. eapply X.
-    clear -X1 H0. simpl; intros. intuition eauto with extends.
-    eapply All_impl; eauto; simpl; intuition eauto with extends.
-  - eapply weakening_env_cumul in H0; eauto. econstructor; eauto.
-Qed.
 
 Definition lift_decl n k (d : context_decl) := map_decl (lift n k) d.
 
@@ -203,8 +36,6 @@ Proof.
   unfold lift_context. now rewrite !List.rev_length, mapi_length, List.rev_length.
 Qed.
 Hint Rewrite lift_context_length : lift.
-
-Require Import Lia.
 
 Lemma lift_context_snoc0 n k Γ d : lift_context n k (d :: Γ) = lift_context n k Γ ,, lift_decl n (#|Γ| + k) d.
 Proof.
@@ -239,21 +70,6 @@ Proof.
   apply mapi_ext. intros. f_equal. rewrite List.rev_length. lia.
 Qed.
 
-Lemma nth_error_app_ge v Γ Γ' : #|Γ'| <= v -> nth_error (Γ ,,, Γ') v = nth_error Γ (v - #|Γ'|).
-Proof.
-  revert v; induction Γ'; simpl; intros.
-  now rewrite Nat.sub_0_r.
-  destruct v. omega.
-  simpl. rewrite IHΓ'; easy.
-Qed.
-
-Lemma nth_error_app_lt v Γ Γ' : v < #|Γ'| -> nth_error (Γ ,,, Γ') v = nth_error Γ' v.
-Proof.
-  revert v; induction Γ'; simpl; intros. easy.
-  destruct v; trivial.
-  simpl. rewrite IHΓ'; easy.
-Qed.
-
 Lemma nth_error_lift_context:
   forall (Γ' Γ'' : context) (v : nat),
     v < #|Γ'| -> forall nth k,
@@ -267,430 +83,39 @@ Proof.
     + simpl. apply IHΓ'; simpl in *; (lia || congruence).
 Qed.
 
-Lemma weaken_safe_nth_ge Γ Γ' v (isdecl : v < #|Γ ,,, Γ'|) Γ'' : #|Γ'| <= v ->
-  { isdecl' : _ &
-  safe_nth (Γ ,,, Γ') (exist (fun n0 : nat => n0 < #|Γ ,,, Γ'|) v isdecl) =
-  safe_nth (Γ ,,, Γ'' ,,, lift_context #|Γ''| 0 Γ') (exist _ (#|Γ''| + v) isdecl') }.
+Lemma nth_error_lift_context_eq:
+  forall (Γ' Γ'' : context) (v : nat) k,
+    nth_error (lift_context #|Γ''| k Γ') v =
+    option_map (lift_decl #|Γ''| (#|Γ'| - S v + k)) (nth_error Γ' v).
 Proof.
-  simpl.
-  assert(#|Γ''| + v < #|Γ ,,, Γ'' ,,, lift_context #|Γ''| 0 Γ'|).
-  rewrite !app_context_length in *. autorewrite with lift. omega.
-  exists H.
-  apply some_inj; rewrite <- !nth_error_safe_nth.
-  rewrite nth_error_app_ge; try easy.
-  rewrite (nth_error_app_ge (_ + v)); rewrite ?lift_context_length; try easy.
-  rewrite nth_error_app_ge; try easy.
+  induction Γ'; intros.
+  - simpl. unfold lift_context; simpl. now rewrite nth_error_nil.
+  - simpl. destruct v; rewrite lift_context_snoc0.
+    + simpl. repeat f_equal; try lia.
+    + simpl. apply IHΓ'; simpl in *; (lia || congruence).
 Qed.
 
-Lemma weaken_safe_nth_lt Γ Γ' v (isdecl : v < #|Γ ,,, Γ'|) Γ'' : v < #|Γ'| ->
-  { isdecl' : _ &
-  safe_nth (Γ ,,, Γ'' ,,, lift_context #|Γ''| 0 Γ') (exist _ v isdecl') =
-  lift_decl #|Γ''| (#|Γ'| - S v)
-       (safe_nth (Γ ,,, Γ') (exist (fun n0 : nat => n0 < #|Γ ,,, Γ'|) v isdecl)) }.
+Lemma weaken_nth_error_ge {Γ Γ' v Γ''} : #|Γ'| <= v ->
+  nth_error (Γ ,,, Γ') v =
+  nth_error (Γ ,,, Γ'' ,,, lift_context #|Γ''| 0 Γ') (#|Γ''| + v).
+Proof.
+  intros Hv.
+  rewrite !nth_error_app_ge, ?lift_context_length. f_equal. lia.
+  rewrite lift_context_length. lia.
+  rewrite lift_context_length. lia. auto.
+Qed.
+
+Lemma weaken_nth_error_lt {Γ Γ' Γ'' v} : v < #|Γ'| ->
+  nth_error (Γ ,,, Γ'' ,,, lift_context #|Γ''| 0 Γ') v =
+  option_map (lift_decl #|Γ''| (#|Γ'| - S v)) (nth_error (Γ ,,, Γ') v).
 Proof.
   simpl. intros Hv.
-  assert(v < #|Γ ,,, Γ'' ,,, lift_context #|Γ''| 0 Γ'|).
-  rewrite !app_context_length in *. autorewrite with lift. omega.
-  exists H.
-  apply some_inj. rewrite <- !nth_error_safe_nth.
-  rewrite nth_error_app_lt. 2:rewrite !app_context_length in H; autorewrite with lift; omega.
-  remember (safe_nth (Γ ,,, Γ') (exist _ v isdecl)) as nth.
-  apply (f_equal Some) in Heqnth. rewrite <- nth_error_safe_nth in Heqnth.
-  rewrite nth_error_app_lt in Heqnth; try easy.
-  replace (#|Γ'| - S v) with (#|Γ'| - S v + 0) by lia.
-  eapply nth_error_lift_context; try lia. eauto.
+  rewrite !nth_error_app_lt.
+  rewrite nth_error_lift_context_eq.
+  do 2 f_equal. lia. lia. now rewrite lift_context_length.
 Qed.
 
-Lemma closedn_lift n k k' t : closedn k t = true -> closedn (k + n) (lift n k' t) = true.
-Proof.
-  revert k.
-  induction t in n, k' |- * using term_forall_list_ind; intros;
-    simpl in *; rewrite ?andb_true_iff in *;
-    rewrite ?map_map_compose, ?compose_on_snd, ?compose_map_def;
-    try (f_equal; apply_spec);  simpl closed in *;
-      try rewrite ?map_length; intuition auto.
-
-  - elim (Nat.leb_spec k' n0); intros. simpl.
-    elim (Nat.ltb_spec); auto. apply Nat.ltb_lt in H. lia.
-    simpl. elim (Nat.ltb_spec); auto. intros.
-    apply Nat.ltb_lt in H. lia.
-  - merge_Forall. rewrite forallb_map. eapply Forall_forallb in H0; intuition eauto.
-  - specialize (IHt2 n (S k') _ H1). eauto.
-  - specialize (IHt2 n (S k') _ H1). eauto.
-  - specialize (IHt3 n (S k') _ H1). eauto.
-  - merge_Forall. rewrite forallb_map. eapply Forall_forallb in H2; intuition eauto.
-  - merge_Forall. rewrite forallb_map. eapply Forall_forallb in H2; intuition eauto.
-    destruct x; unfold test_snd, compose, on_snd; simpl. eapply H1. auto.
-  - merge_Forall. rewrite forallb_map. eapply Forall_forallb in H0; intuition eauto.
-    unfold test_def, compose, map_def in *. simpl.
-    rewrite !andb_true_iff in *. intuition auto.
-    rewrite Nat.add_assoc. eauto.
-  - merge_Forall. rewrite forallb_map. eapply Forall_forallb in H0; intuition eauto.
-    unfold test_def, compose, map_def in *. simpl.
-    rewrite !andb_true_iff in *. intuition auto.
-    rewrite Nat.add_assoc. eauto.
-Qed.
-
-Lemma closedn_lift_inv n k k' t : k <= k' ->
-                                   closedn (k' + n) (lift n k t) = true ->
-                                   closedn k' t = true.
-Proof.
-  induction t in n, k, k' |- * using term_forall_list_ind; intros;
-    simpl in *; rewrite ?andb_true_iff in *;
-    rewrite ?map_map_compose, ?compose_on_snd, ?compose_map_def;
-    try (f_equal; apply_spec);  simpl closed in *;
-      try rewrite ?map_length; intuition eauto 2.
-
-  - revert H0.
-    elim (Nat.leb_spec k n0); intros. simpl in *.
-    elim (Nat.ltb_spec); auto. apply Nat.ltb_lt in H1. intros. lia.
-    revert H1. simpl. elim (Nat.ltb_spec); auto. intros. apply Nat.ltb_lt. lia.
-    intros; discriminate.
-  - rewrite forallb_map in H1. merge_Forall. eapply Forall_forallb; eauto.
-    simpl; intuition eauto.
-  - specialize (IHt2 n (S k) (S k')). eauto with arith.
-  - specialize (IHt2 n (S k) (S k')). eauto with arith.
-  - specialize (IHt3 n (S k) (S k')). eauto with arith.
-  - rewrite forallb_map in H3. merge_Forall. eapply Forall_forallb; eauto. simpl; intuition eauto.
-  - rewrite forallb_map in H3. merge_Forall. eapply Forall_forallb; eauto. simpl; intuition eauto.
-    destruct x; unfold test_snd, compose, on_snd in *; simpl in *; eauto.
-  - rewrite forallb_map in H1. merge_Forall. eapply Forall_forallb; intuition eauto.
-    unfold test_def, compose, map_def in *. simpl in *.
-    rewrite !andb_true_iff in *. rewrite !map_length in *. intuition eauto 2.
-    rewrite Nat.add_assoc in H5. specialize (H4 n (#|m| + k) (#|m| + k')). forward H4 by lia.
-    apply H4. auto.
-  - rewrite forallb_map in H1. merge_Forall. eapply Forall_forallb; intuition eauto.
-    unfold test_def, compose, map_def in *. simpl in *.
-    rewrite !andb_true_iff in *. rewrite !map_length in *. intuition eauto 2.
-    rewrite Nat.add_assoc in H5. specialize (H4 n (#|m| + k) (#|m| + k')). forward H4 by lia.
-    apply H4. auto.
-Qed.
-
-Lemma closedn_mkApps k f u:
-  closedn k f = true -> forallb (closedn k) u = true ->
-  closedn k (mkApps f u) = true.
-Proof.
-  intros Hf Hu.
-  induction u; simpl; auto.
-  destruct f; simpl in *; try rewrite Hf, Hu; auto.
-  rewrite forallb_app. simpl. rewrite Hu.
-  rewrite andb_assoc. now rewrite Hf.
-Qed.
-
-Lemma closedn_mkApps_inv k f u:
-  closedn k (mkApps f u) = true ->
-  closedn k f && forallb (closedn k) u = true.
-Proof.
-  induction u; simpl; auto.
-  - now rewrite andb_true_r.
-  - intros. destruct f; simpl in *; auto.
-    rewrite forallb_app in H. simpl in H.
-    now rewrite andb_assoc in H.
-Qed.
-
-Lemma closedn_parsubst s k k' t :
-  forallb (closedn k) s = true -> closedn (k + k' + #|s|) t = true ->
-  closedn (k + k') (parsubst s k' t) = true.
-Proof.
-  induction t in k' |- * using term_forall_list_ind; intros;
-    simpl in *; rewrite ?andb_true_iff in *;
-    rewrite ?map_map_compose, ?compose_on_snd, ?compose_map_def;
-    try (f_equal; apply_spec);  simpl closed in *;
-      try rewrite ?map_length; intuition auto.
-
-  - elim (Nat.leb_spec k' n); intros. simpl.
-    apply Nat.ltb_lt in H0.
-    destruct nth_error eqn:Heq.
-    -- eapply closedn_lift. eapply forallb_Forall in H; eauto. 2:{ intros. apply H2. }
-       now eapply nth_error_forall in Heq; simpl; eauto; simpl in *.
-    -- simpl. elim (Nat.ltb_spec); auto. intros.
-       apply nth_error_None in Heq. lia.
-    -- simpl. apply Nat.ltb_lt in H0.
-       apply Nat.ltb_lt. lia.
-
-  - merge_Forall. rewrite forallb_map.
-    eapply Forall_forallb; eauto. unfold compose; intuition eauto.
-  - specialize (IHt2 (S k') H).
-    rewrite <- Nat.add_succ_comm in IHt2. eauto.
-  - specialize (IHt2 (S k') H).
-    rewrite <- Nat.add_succ_comm in IHt2. eauto.
-  - specialize (IHt3 (S k') H).
-    rewrite <- Nat.add_succ_comm in IHt3. eauto.
-  - merge_Forall.
-    rewrite closedn_mkApps. eauto.
-    now specialize (IHt k' H0).
-    rewrite forallb_map. eapply Forall_forallb; eauto. simpl; intuition eauto.
-  - merge_Forall. rewrite forallb_map. eapply Forall_forallb; eauto.
-    simpl. intros [n trm]. unfold test_snd, on_snd, compose. intuition eauto.
-  - merge_Forall. rewrite forallb_map. eapply Forall_forallb; eauto. simpl; intuition eauto.
-    unfold test_def, compose, map_def in *. simpl.
-    rewrite !andb_true_iff in *. intuition auto.
-    rewrite Nat.add_assoc.
-    specialize (H4 (#|m| + k')).
-    rewrite <- H4; eauto.
-    f_equal; lia. rewrite <- H5. f_equal; lia.
-  - merge_Forall. rewrite forallb_map. eapply Forall_forallb; eauto. simpl; intuition eauto.
-    unfold test_def, compose, map_def in *. simpl.
-    rewrite !andb_true_iff in *. intuition auto.
-    rewrite Nat.add_assoc.
-    specialize (H4 (#|m| + k')).
-    rewrite <- H4; eauto.
-    f_equal; lia. rewrite <- H5. f_equal; lia.
-Qed.
-
-Lemma closedn_substl s k t :
-  forallb (closedn k) s = true -> closedn (k + #|s|) t = true ->
-  closedn k (substl s t) = true.
-Proof.
-  unfold substl.
-  intros.
-  generalize (closedn_parsubst s k 0 t H).
-  rewrite Nat.add_0_r. eauto.
-Qed.
-
-Lemma closedn_subst_instance_constr k t u :
-  closedn k (UnivSubst.subst_instance_constr u t) = closedn k t.
-Proof.
-  revert k.
-  induction t in |- * using term_forall_list_ind; intros;
-    simpl in *; rewrite ?andb_true_iff in *;
-    rewrite ?map_map_compose, ?compose_on_snd, ?compose_map_def;
-    try solve [repeat (f_equal; eauto)];  simpl closed in *;
-      try rewrite ?map_length; intuition auto.
-
-  - rewrite forallb_map; eapply Forall_forallb_eq_forallb; eauto.
-  - rewrite forallb_map. f_equal; eauto using Forall_forallb_eq_forallb.
-  - red in H. rewrite forallb_map. f_equal; eauto using Forall_forallb_eq_forallb.
-    f_equal; eauto.
-  - red in H. rewrite forallb_map.
-    eapply Forall_forallb_eq_forallb; eauto.
-    unfold test_def, compose, map_def. simpl.
-    do 3 (f_equal; intuition eauto).
-  - red in H. rewrite forallb_map.
-    eapply Forall_forallb_eq_forallb; eauto.
-    unfold test_def, compose, map_def. simpl.
-    do 3 (f_equal; intuition eauto).
-Qed.
-
-Definition weaken_env_prop `{checker_flags}
-           (P : global_context -> context -> option term -> term -> Type) :=
-  forall Σ Σ', wf Σ' -> extends Σ Σ' -> forall Γ t T, P Σ Γ t T -> P Σ' Γ t T.
-
-Lemma weakening_on_global_decl `{checker_flags} P Σ Σ' decl :
-  weaken_env_prop P ->
-  wf Σ' -> extends Σ Σ' ->
-  on_global_decl P Σ decl ->
-  on_global_decl P Σ' decl.
-Proof.
-  unfold weaken_env_prop.
-  intros HPΣ wfΣ' Hext Hdecl.
-  destruct decl. destruct c. destruct cst_body. simpl in *.
-  red in Hdecl |- *. simpl in *.
-  eapply HPΣ; eauto.
-  eapply HPΣ; eauto.
-  simpl in *.
-  do 2 red in Hdecl. eapply Alli_impl; eauto.
-  intros.
-  destruct X. constructor.
-  unfold on_type in *; eauto.
-  unfold on_constructors in *. eapply All_impl; eauto.
-  intros [[id t] ar]. unfold on_constructor, on_type in *; eauto.
-  destruct decompose_prod_assum. intuition.
-  eapply All_impl; eauto. intros [id trm].
-  unfold on_projection, on_type; eauto.
-Qed.
-
-Lemma weakening_env_lookup_on_global_env `{checker_flags} P Σ Σ' c decl :
-  weaken_env_prop P ->
-  wf Σ' -> extends Σ Σ' -> on_global_env P Σ ->
-  lookup_env (fst Σ) c = Some decl ->
-  on_global_decl P Σ' decl.
-Proof.
-  intros HP wfΣ Hext HΣ. destruct Σ as [Σ graph].
-  red in HΣ. simpl in *.
-  induction HΣ; simpl. congruence.
-  destruct ident_eq. intros [= ->].
-  eapply weakening_on_global_decl. eauto. eauto. 2:{ eapply o. }
-  destruct Hext. simpl in *. rewrite H0.
-  exists ((x ++ [decl])%list). simpl.
-  now rewrite <- app_assoc.
-
-  apply IHHΣ.
-  destruct Hext as [Σ'' ->]. simpl. red.
-  exists (Σ'' ++ [d])%list. simpl.
-  now rewrite <- app_assoc.
-Qed.
-
-Lemma weaken_lookup_on_global_env `{checker_flags} P Σ c decl :
-  weaken_env_prop P ->
-  wf Σ -> on_global_env P Σ ->
-  lookup_env (fst Σ) c = Some decl ->
-  on_global_decl P Σ decl.
-Proof.
-  intros. eapply weakening_env_lookup_on_global_env; eauto.
-  exists []; simpl; destruct Σ; eauto.
-Qed.
-
-Lemma declared_minductive_inv `{checker_flags} Σ P ind mdecl :
-  weaken_env_prop (lift_typing P) ->
-  wf Σ -> Forall_decls_typing P Σ ->
-  declared_minductive (fst Σ) ind mdecl ->
-  on_inductive (lift_typing P) Σ ind
-               (polymorphic_instance (ind_universes mdecl))
-               (ind_npars mdecl) (ind_bodies mdecl).
-Proof.
-  intros.
-  eapply weaken_lookup_on_global_env in X1; eauto. apply X1.
-Qed.
-
-Lemma declared_inductive_inv `{checker_flags} Σ P ind mdecl idecl :
-  weaken_env_prop (lift_typing P) ->
-  wf Σ -> Forall_decls_typing P Σ ->
-  declared_inductive (fst Σ) ind mdecl idecl ->
-  on_ind_body (lift_typing P) Σ (inductive_mind ind)
-               (polymorphic_instance (ind_universes mdecl))
-               (ind_npars mdecl) (arities_context (ind_bodies mdecl)) (inductive_ind ind) idecl.
-Proof.
-  intros.
-  destruct H0 as [Hmdecl Hidecl].
-  eapply declared_minductive_inv in Hmdecl; eauto.
-  eapply nth_error_alli in Hidecl; eauto.
-  apply Hidecl.
-Qed.
-
-Lemma typecheck_closed `{cf : checker_flags} :
-  env_prop (fun Σ Γ t T =>
-              closedn #|Γ| t && closedn #|Γ| T = true).
-Proof.
-  assert(weaken_env_prop (lift_typing (fun (_ : global_context) (Γ : context) (t T : term) =>
-                                         closedn #|Γ| t && closedn #|Γ| T = true))).
-  { repeat red. intros. destruct t; red in X0; eauto. }
-
-  apply typing_ind_env; intros; simpl; rewrite ?andb_true_iff in *; try solve [intuition auto].
-  - elim (Nat.ltb_spec n #|Γ|); intuition.
-    eapply (All_local_env_lookup isdecl) in H. red in H.
-    destruct decl_body.
-    -- rewrite andb_true_iff in H; intuition.
-       rewrite skipn_length in H2 by lia.
-       eapply (closedn_lift (S n)) in H2.
-       assert(#|Γ| - S n + S n = #|Γ|) by lia.
-       rewrite H in H2. apply H2.
-    -- destruct H as [s Hs].
-       rewrite andb_true_iff in Hs; intuition.
-       rewrite skipn_length in H by lia.
-       eapply (closedn_lift (S n)) in H.
-       assert(#|Γ| - S n + S n = #|Γ|) by lia.
-       rewrite H2 in H. apply H.
-
-  - destruct H. rewrite and_assoc. split. auto.
-    clear X0 H H0 H1.
-    induction X1; simpl. intuition auto.
-    rewrite andb_true_iff in *. destruct p0. rewrite H.
-    rewrite <- andb_true_iff. simpl.
-    apply IHX1. unfold subst.
-    pose proof (closedn_parsubst [hd] #|Γ| 0). rewrite Nat.add_0_r in H1.
-    apply H1. simpl. now rewrite H.
-    simpl. simpl in p. rewrite andb_true_iff in p. intuition auto.
-    rewrite Nat.add_1_r. auto.
-
-  - rewrite closedn_subst_instance_constr.
-    eapply lookup_on_global_env in H; eauto.
-    destruct H as [Σ' [HΣ' IH]].
-    repeat red in IH. destruct decl, cst_body. simpl in *.
-    rewrite andb_true_iff in IH. intuition.
-    eauto using closed_upwards with arith.
-    simpl in *.
-    repeat red in IH. destruct IH as [s Hs].
-    rewrite andb_true_iff in Hs. intuition.
-    eauto using closed_upwards with arith.
-
-  - rewrite closedn_subst_instance_constr.
-    eapply declared_inductive_inv in X0; eauto.
-    apply onArity in X0. repeat red in X0.
-    destruct X0 as [s Hs]. rewrite andb_true_iff in Hs.
-    intuition eauto using closed_upwards with arith.
-
-  - destruct isdecl as [Hidecl Hcdecl].
-    eapply declared_inductive_inv in X0; eauto.
-    apply onConstructors in X0. repeat red in X0.
-    eapply nth_error_all in Hcdecl; eauto.
-    repeat red in Hcdecl.
-    destruct Hcdecl as [s Hs]. rewrite andb_true_iff in Hs.
-    destruct Hs as [Hdecl _].
-    unfold type_of_constructor.
-    apply closedn_substl.
-    unfold inds. clear. simpl. induction #|ind_bodies mdecl|. constructor.
-    simpl. now rewrite IHn.
-    rewrite inds_length. unfold arities_context in Hdecl.
-    rewrite rev_map_length in Hdecl.
-    rewrite closedn_subst_instance_constr.
-    eauto using closed_upwards with arith.
-
-  - intuition auto.
-    eapply Forall_forallb; eauto.
-    eapply Forall2_Forall_left; eauto.
-    simpl; intros. destruct X4. rewrite andb_true_iff in e. destruct e.
-    apply H7. simpl; intros. eauto.
-    apply closedn_mkApps; auto.
-    rewrite forallb_app. simpl. rewrite H6.
-    rewrite forallb_skipn; auto.
-    now apply closedn_mkApps_inv in H11.
-
-  - intuition. subst ty.
-    apply closedn_substl.
-    simpl. apply closedn_mkApps_inv in H2.
-    rewrite forallb_rev, H1. apply H2.
-    rewrite closedn_subst_instance_constr.
-    destruct isdecl as [isdecl Hpdecl].
-    eapply declared_inductive_inv in isdecl; eauto.
-    apply onProjections in isdecl.
-    destruct decompose_prod_assum eqn:Heq.
-    destruct isdecl as [Hc isdecl].
-    eapply nth_error_all in isdecl; eauto.
-    destruct isdecl as [s Hs]. simpl in *.
-    forward Hc. intro. rewrite H in Hpdecl; destruct (snd p); discriminate.
-    rewrite <- Hc in H0. rewrite <- H0 in Hs.
-    rewrite andb_true_r in Hs. rewrite List.rev_length.
-    eauto using closed_upwards with arith.
-
-  - split. eapply All_forallb; eauto.
-    simpl; eauto. intros. intuition.
-    destruct x; simpl in *.
-    unfold test_def. simpl.
-    rewrite andb_true_iff in *. destruct b.
-    split.
-    rewrite app_context_length in *. rewrite Nat.add_comm in *.
-    eapply closedn_lift_inv in H0; eauto. lia.
-    subst types.
-    now rewrite app_context_length, fix_context_length in H.
-    subst ty.
-    eapply (All_safe_nth isdecl) in X1. simpl in X1.
-    intuition.
-    rewrite !andb_true_iff in b. intuition.
-    subst types. rewrite app_context_length in H0.
-    rewrite Nat.add_comm in H0.
-    now eapply closedn_lift_inv in H0.
-
-  - split. eapply All_forallb; eauto.
-    simpl; eauto. intros. intuition.
-    destruct x; simpl in *.
-    unfold test_def. simpl.
-    rewrite andb_true_iff in *. destruct b.
-    split.
-    rewrite app_context_length in *. rewrite Nat.add_comm in *.
-    eapply closedn_lift_inv in H0; eauto. lia.
-    subst types.
-    now rewrite app_context_length, fix_context_length in H.
-    subst ty.
-    eapply (All_safe_nth isdecl) in X1. simpl in X1.
-    intuition.
-    rewrite !andb_true_iff in b. intuition.
-    subst types. rewrite app_context_length in H0.
-    rewrite Nat.add_comm in H0.
-    now eapply closedn_lift_inv in H0.
-Qed.
-
-Lemma lift_simpl (Γ'' Γ' : context) i t : i < #|Γ'| ->
+Lemma lift_simpl {Γ'' Γ' : context} {i t} : i < #|Γ'| ->
   lift0 (S i) (lift #|Γ''| (#|Γ'| - S i) t) = lift #|Γ''| #|Γ'| (lift0 (S i) t).
 Proof.
   intros. assert (#|Γ'| = S i + (#|Γ'| - S i)) by easy.
@@ -706,29 +131,7 @@ Proof.
   rewrite nth_map; simpl; auto.
 Qed.
 
-Definition lift_subst n k s :=
-  List.fold_right (fun t l => lift n (List.length l + k) t :: l) [] s.
-
-Lemma lift_subst_length n k s : #|lift_subst n k s| = #|s|.
-Proof.
-  induction s in n, k |- *; simpl; auto.
-Qed.
-
-Lemma fix_subst_length mfix : #|fix_subst mfix| = #|mfix|.
-Proof.
-  unfold fix_subst. generalize (tFix mfix). intros.
-  induction mfix; simpl; auto.
-Qed.
-
-Lemma cofix_subst_length mfix : #|cofix_subst mfix| = #|mfix|.
-Proof.
-  unfold cofix_subst. generalize (tCoFix mfix). intros.
-  induction mfix; simpl; auto.
-Qed.
-
-Require Import Compare_dec Lia.
-
-Lemma parsubst_empty k a : Ast.wf a -> parsubst [] k a = a.
+Lemma parsubst_empty k a : Ast.wf a -> subst [] k a = a.
 Proof.
   induction 1 in k |- * using term_wf_forall_list_ind; simpl; try congruence;
     try solve [f_equal; eauto; apply_spec; eauto].
@@ -792,27 +195,8 @@ Hint Resolve lift_is_constructor.
 
 Hint Rewrite UnivSubst.lift_subst_instance_constr : lift.
 Hint Rewrite lift_mkApps : lift.
-Hint Rewrite distr_lift_subst : lift.
+Hint Rewrite distr_lift_subst distr_lift_subst10 : lift.
 Hint Rewrite lift_iota_red : lift.
-
-Definition map_constant_body f decl :=
-  {| cst_type := f decl.(cst_type);
-     cst_body := option_map f decl.(cst_body);
-     cst_universes := decl.(cst_universes) |}.
-
-Lemma map_cst_type f decl : f (cst_type decl) = cst_type (map_constant_body f decl).
-Proof. destruct decl; reflexivity. Qed.
-
-Lemma map_cst_body f decl : option_map f (cst_body decl) = cst_body (map_constant_body f decl).
-Proof. destruct decl; reflexivity. Qed.
-
-Lemma map_dtype {A B : Set} (f : A -> B) (g : A -> B) (d : def A) :
-  f (dtype d) = dtype (map_def f g d).
-Proof. destruct d; reflexivity. Qed.
-
-Lemma map_dbody {A B : Set} (f : A -> B) (g : A -> B) (d : def A) :
-  g (dbody d) = dbody (map_def f g d).
-Proof. destruct d; reflexivity. Qed.
 
 Lemma lift_declared_constant `{checker_flags} Σ cst decl n k :
   wf Σ ->
@@ -843,45 +227,6 @@ Proof.
   apply (lift_closed n k) in ccst. unfold map_constant_body. simpl.
   rewrite ccst. reflexivity. lia. auto. constructor.
 Qed.
-
-Definition map_one_inductive_body mind u arities f n m :=
-  match m with
-  | Build_one_inductive_body ind_name ind_type ind_kelim ind_ctors ind_projs =>
-    let '(ctx, _) := decompose_prod_assum [] (f [] ind_type) in
-    let indty := mkApps (tInd (mkInd mind n) u) (to_extended_list ctx) in
-    Build_one_inductive_body ind_name
-                             (f [] ind_type)
-                             ind_kelim
-                             (map (on_pi2 (f arities)) ind_ctors)
-                             (map (on_snd (f (ctx ,, vass (nNamed ind_name) indty))) ind_projs)
-  end.
-
-Definition map_mutual_inductive_body mind f m :=
-  match m with
-  | Build_mutual_inductive_body ind_npars ind_bodies ind_universes =>
-    let arities := arities_context ind_bodies in
-    let u := polymorphic_instance ind_universes in
-    Build_mutual_inductive_body
-      ind_npars
-      (mapi (map_one_inductive_body mind u arities f) ind_bodies)
-      ind_universes
-  end.
-
-Lemma ind_type_map f arities mind u n oib :
-  ind_type (map_one_inductive_body mind u arities f n oib) = f [] (ind_type oib).
-Proof. destruct oib. simpl. destruct decompose_prod_assum. reflexivity. Qed.
-
-Lemma ind_ctors_map f arities mind u n oib :
-  ind_ctors (map_one_inductive_body mind u arities f n oib) =
-  map (on_pi2 (f arities)) (ind_ctors oib).
-Proof. destruct oib; simpl; destruct decompose_prod_assum; reflexivity. Qed.
-
-Lemma ind_projs_map f mind u arities n oib :
-  ind_projs (map_one_inductive_body mind u arities f n oib) =
-  let '(ctx, _) := decompose_prod_assum [] (f [] oib.(ind_type)) in
-  map (on_snd (f (ctx ,, vass (nNamed oib.(ind_name))
-      (mkApps (tInd (mkInd mind n) u) (to_extended_list ctx))))) (ind_projs oib).
-Proof. destruct oib; simpl. destruct decompose_prod_assum. simpl. reflexivity. Qed.
 
 Definition lift_mutual_inductive_body n k mind m :=
   map_mutual_inductive_body mind (fun Γ => lift n (#|Γ| + k)) m.
@@ -987,6 +332,37 @@ Proof.
   now rewrite substl_inds_lift.
 Qed.
 
+Lemma lift_declared_projection `{checker_flags} Σ c mdecl idecl pdecl n k :
+  wf Σ ->
+  declared_projection (fst Σ) mdecl idecl c pdecl ->
+  on_snd (lift n (S (ind_npars mdecl + k))) pdecl = pdecl.
+Proof.
+  unfold declared_projection. destruct c as [[i k'] ci]. intros wfΣ [Hidecl Hcdecl].
+  simpl in *.
+  pose proof Hidecl. destruct H0 as [Hmdecl Hidecl'].
+  eapply lookup_on_global_env in Hmdecl; eauto.
+  destruct Hmdecl as [Σ' [wfΣ' ongdecl]].
+  red in ongdecl. red in ongdecl.
+  eapply nth_error_alli in Hidecl'; eauto.
+  apply onProjections in Hidecl'.
+  destruct decompose_prod_assum eqn:Heq.
+  destruct Hidecl' as [Hpars _].
+  destruct Σ. eapply (lift_declared_inductive _ _ _ _ n k) in Hidecl; eauto.
+  destruct pdecl as [id t'].
+  destruct idecl; simpl in *.
+  destruct (decompose_prod_assum _ _) eqn:Heq'.
+  injection Hidecl.
+  intros.
+  rewrite <- H2 in Heq. rewrite Heq in Heq'. injection Heq'. intros <- <-.
+  forward Hpars. destruct ind_projs; destruct ci; discriminate.
+  rewrite Hpars in H0.
+  pose proof Hcdecl as Hcdecl'.
+  rewrite <- H0 in Hcdecl.
+  rewrite nth_error_map in Hcdecl; eauto.
+  rewrite Hcdecl' in Hcdecl. simpl in Hcdecl.
+  congruence.
+Qed.
+
 Lemma lift_fix_context:
   forall (mfix : list (def term)) (n k : nat),
     fix_context (map (map_def (lift n k) (lift n (#|mfix| + k))) mfix) = lift_context n k (fix_context mfix).
@@ -997,6 +373,8 @@ Proof.
   rewrite (lift_context_alt n k (fix_context mfix)).
   unfold lift_decl. now rewrite mapi_length, fix_context_length.
 Qed.
+
+Hint Rewrite <- lift_fix_context : lift.
 
 Lemma All_local_env_lift `{checker_flags} (P Q : global_context -> context -> term -> term -> Type) Σ c n k :
   All_local_env Q Σ c ->
@@ -1028,15 +406,16 @@ Proof.
 Qed.
 
 Lemma lift_instantiate_params n k args t :
-  lift n k (instantiate_params args t) =
+  option_map (lift n k) (instantiate_params args t) =
   instantiate_params (map (lift n k) args) (lift n k t).
 Proof.
   induction args in t, n, k |- *. reflexivity.
   simpl. destruct t; simpl; try congruence.
   - now destruct (Nat.leb k n0).
-  - rewrite <- distr_lift_subst. eauto.
-  - rewrite <- distr_lift_subst. eauto.
+  - rewrite IHargs. f_equal. apply distr_lift_subst.
+  - rewrite IHargs; f_equal. apply distr_lift_subst.
 Qed.
+Hint Rewrite lift_instantiate_params : lift.
 
 (* bug eauto with let .. in hypothesis failing *)
 Lemma lift_decompose_prod_assum_rec ctx t n k :
@@ -1066,6 +445,7 @@ Lemma decompose_app_lift n k t f a :
   decompose_app t = (f, a) -> decompose_app (lift n k t) = (lift n k f, map (lift n k) a).
 Proof. destruct t; simpl; intros [= <- <-]; try reflexivity.
        simpl. now destruct (Nat.leb k n0). Qed.
+Hint Rewrite decompose_app_lift using auto : lift.
 
 Lemma lift_it_mkProd_or_LetIn n k ctx t :
   lift n k (it_mkProd_or_LetIn ctx t) =
@@ -1076,45 +456,16 @@ Proof.
   simpl. destruct decl_body. now rewrite IHctx.
   pose (lift_context_snoc n k ctx a). simpl. now rewrite IHctx.
 Qed.
+Hint Rewrite lift_it_mkProd_or_LetIn : lift.
 
 Lemma to_extended_list_lift n k c :
   to_extended_list (lift_context n k c) = to_extended_list c.
 Proof.
-  unfold to_extended_list. generalize 0 at 3 6. generalize (@nil term) at 1 2.
+  unfold to_extended_list. generalize 0. generalize (@nil term) at 1 2.
   induction c in n, k |- *; simpl; intros. reflexivity.
   rewrite lift_context_snoc0. unfold snoc. simpl.
   destruct a. destruct decl_body. unfold lift_decl, map_decl. simpl.
   now rewrite IHc. simpl. apply IHc.
-Qed.
-
-Fixpoint reln (l : list term) (p : nat) (Γ0 : list context_decl) {struct Γ0} : list term :=
-  match Γ0 with
-  | [] => l
-  | {| decl_body := Some _ |} :: hyps => reln l (p + 1) hyps
-  | {| decl_body := None |} :: hyps => reln (tRel p :: l) (p + 1) hyps
-  end.
-
-Lemma reln_list_lift_above l p Γ :
-  Forall (fun x => exists n, x = tRel n /\ n < p + length Γ) l ->
-  Forall (fun x => exists n, x = tRel n /\ n < p + length Γ) (reln l p Γ).
-Proof.
-  induction Γ in p, l |- *. simpl. auto.
-  intros. destruct a. destruct decl_body. simpl.
-  specialize (IHΓ l (S p)). rewrite <- Nat.add_succ_comm, Nat.add_1_r.
-  eapply IHΓ. simpl in *. rewrite <- Nat.add_succ_comm in H. auto.
-  simpl in *.
-  specialize (IHΓ (tRel p :: l) (S p)). rewrite <- Nat.add_succ_comm, Nat.add_1_r.
-  eapply IHΓ. simpl in *. rewrite <- Nat.add_succ_comm in H. auto.
-  simpl in *.
-  constructor. exists p. intuition lia. auto.
-Qed.
-
-Lemma to_extended_list_lift_above Γ :
-  Forall (fun x => exists n, x = tRel n /\ n < length Γ) (to_extended_list Γ).
-Proof.
-  pose (reln_list_lift_above [] 0 Γ).
-  unfold to_extended_list.
-  forward f. constructor. apply f.
 Qed.
 
 Lemma to_extended_list_map_lift:
@@ -1145,20 +496,25 @@ Proof.
   pose proof (lift_destArity [] pty n k wfpty); trivial. simpl in H.
   unfold lift_context in H. simpl in H. rewrite H. clear H.
   destruct destArity as [[ctx' s'] | ]; try congruence.
-  intros [= -> -> -> <-].
-  f_equal. f_equal.
-  unfold build_branches_type. simpl.
+  assert(forall brs,
+         build_branches_type ind mdecl idecl args u p = brs ->
+         (build_branches_type ind mdecl
+         (map_one_inductive_body (inductive_mind ind) (polymorphic_instance (ind_universes mdecl))
+            (arities_context (ind_bodies mdecl)) (fun ctx0 : list context_decl => lift n (#|ctx0| + k))
+            (inductive_ind ind) idecl) (map (lift n k) args) u (lift n k p)) =
+         map (option_map (on_snd (lift n k))) brs).
+  unfold build_branches_type. simpl. intros brs. intros <-.
   rewrite ind_ctors_map.
   rewrite mapi_map, map_mapi. f_equal. extensionality i. extensionality x.
   destruct x as [[id t] arity]. simpl.
   rewrite <- UnivSubst.lift_subst_instance_constr.
   rewrite substl_inds_lift.
   rewrite <- lift_instantiate_params.
-  remember (instantiate_params _ _) as instparams.
-  epose proof (lift_decompose_prod_assum instparams n k).
-  destruct (decompose_prod_assum [] instparams).
+  destruct (instantiate_params _ _) eqn:Heqip. simpl.
+  epose proof (lift_decompose_prod_assum t0 n k).
+  destruct (decompose_prod_assum [] t0).
   rewrite <- H.
-  destruct (decompose_app t0) as [fn arg] eqn:?.
+  destruct (decompose_app t1) as [fn arg] eqn:?.
   rewrite (decompose_app_lift _ _ _ fn arg); auto. simpl.
   destruct (chop _ arg) eqn:Heqchop. eapply chop_map in Heqchop.
   rewrite Heqchop. clear Heqchop.
@@ -1167,6 +523,11 @@ Proof.
   rewrite !lift_mkApps, !map_app, lift_context_length.
   rewrite permute_lift by lia. repeat f_equal.
   now rewrite to_extended_list_lift, <- to_extended_list_map_lift.
+  simpl. reflexivity.
+  specialize (H _ eq_refl). rewrite H. clear H.
+  rewrite map_option_out_map_option_map.
+  destruct (map_option_out (build_branches_type _ _ _ _ _ _)).
+  intros [= -> -> -> <-]. reflexivity. congruence.
 Qed.
 
 Lemma weakening_red1 `{CF:checker_flags} Σ Γ Γ' Γ'' M N :
@@ -1182,14 +543,13 @@ Proof.
 
   - elim (leb_spec_Set); intros Hn.
     + rewrite simpl_lift; try lia. rewrite Nat.add_succ_r.
-      destruct (weaken_safe_nth_ge _ _ _ isdecl Γ'' Hn) as [isdecl' Heq].
-      rewrite Heq in H.
-      unshelve econstructor; eauto.
-    + destruct (weaken_safe_nth_lt _ _ _ isdecl Γ'' Hn) as [isdecl' Heq].
-      rewrite <- lift_simpl by easy.
+      econstructor; eauto.
+      erewrite (weaken_nth_error_ge Hn) in H. eauto.
+
+    + rewrite <- lift_simpl by easy.
       econstructor.
-      apply (f_equal decl_body) in Heq.
-      rewrite Heq. unfold lift_decl. simpl. now rewrite H.
+      rewrite (weaken_nth_error_lt Hn).
+      now unfold lift_decl; rewrite option_map_decl_body_lift_decl, H.
 
   - econstructor.
     eauto. rewrite H0. f_equal.
@@ -1347,37 +707,6 @@ Proof.
   eapply lift_eq_context in H0. eapply H0.
 Qed.
 
-Lemma lift_declared_projection `{checker_flags} Σ c mdecl idecl pdecl n k :
-  wf Σ ->
-  declared_projection (fst Σ) mdecl idecl c pdecl ->
-  on_snd (lift n (S (ind_npars mdecl + k))) pdecl = pdecl.
-Proof.
-  unfold declared_projection. destruct c as [[i k'] ci]. intros wfΣ [Hidecl Hcdecl].
-  simpl in *.
-  pose proof Hidecl. destruct H0 as [Hmdecl Hidecl'].
-  eapply lookup_on_global_env in Hmdecl; eauto.
-  destruct Hmdecl as [Σ' [wfΣ' ongdecl]].
-  red in ongdecl. red in ongdecl.
-  eapply nth_error_alli in Hidecl'; eauto.
-  apply onProjections in Hidecl'.
-  destruct decompose_prod_assum eqn:Heq.
-  destruct Hidecl' as [Hpars _].
-  destruct Σ. eapply (lift_declared_inductive _ _ _ _ n k) in Hidecl; eauto.
-  destruct pdecl as [id t'].
-  destruct idecl; simpl in *.
-  destruct (decompose_prod_assum _ _) eqn:Heq'.
-  injection Hidecl.
-  intros.
-  rewrite <- H2 in Heq. rewrite Heq in Heq'. injection Heq'. intros <- <-.
-  forward Hpars. destruct ind_projs; destruct ci; discriminate.
-  rewrite Hpars in H0.
-  pose proof Hcdecl as Hcdecl'.
-  rewrite <- H0 in Hcdecl.
-  rewrite nth_error_map in Hcdecl; eauto.
-  rewrite Hcdecl' in Hcdecl. simpl in Hcdecl.
-  congruence.
-Qed.
-
 Lemma weakening_typing `{cf : checker_flags} Σ Γ Γ' Γ'' (t : term) :
   wf Σ ->
   wf_local Σ (Γ ,,, Γ') ->
@@ -1397,17 +726,16 @@ Proof.
     intros Σ wfΣ Γ0 wfΓ0; intros; subst Γ0; simpl in *; try solve [econstructor; eauto].
 
   - elim (leb_spec_Set); intros Hn.
-    + destruct (weaken_safe_nth_ge _ _ _ isdecl Γ'' Hn) as [isdecl' ->].
-      rewrite simpl_lift; try omega. rewrite Nat.add_succ_r.
+    + rewrite simpl_lift; try omega. rewrite Nat.add_succ_r.
       constructor. auto.
-    + destruct (weaken_safe_nth_lt _ _ _ isdecl Γ'' Hn) as [isdecl' H'].
-      apply (f_equal decl_type) in H'.
-      unfold lift_decl in H'. simpl in H'.
-      assert (forall t, lift0 (S n) (lift #|Γ''| (#|Γ'| - S n) t) = lift #|Γ''| #|Γ'| (lift0 (S n) t)).
+      now rewrite <- (weaken_nth_error_ge Hn).
+    + assert (forall t, lift0 (S n) (lift #|Γ''| (#|Γ'| - S n) t) = lift #|Γ''| #|Γ'| (lift0 (S n) t)).
       intros. assert (#|Γ'| = S n + (#|Γ'| - S n)) by easy.
-      rewrite H at 2.
+      rewrite H0 at 2.
       rewrite <- permute_lift; try easy.
-      rewrite <- H. rewrite <- H'. constructor. auto.
+      rewrite <- H0.
+      rewrite map_decl_type. constructor; auto.
+      now rewrite (weaken_nth_error_lt Hn), H.
 
   - econstructor; auto.
     specialize (X2 Γ (Γ' ,, vass n t) Γ'').
@@ -1441,7 +769,7 @@ Proof.
     change (tProd na (lift #|Γ''| #|Γ'| A) (lift #|Γ''| (S #|Γ'|) B))
       with (lift #|Γ''| #|Γ'| (tProd na A B)).
     eapply weakening_cumul; eauto. auto.
-    rewrite distr_lift_subst in IHX1. apply IHX1.
+    rewrite distr_lift_subst10 in IHX1. apply IHX1.
 
   - autorewrite with lift.
     rewrite map_cst_type. constructor; auto.
@@ -1503,13 +831,12 @@ Proof.
     rewrite lift_mkApps in X1. eapply X1.
     now rewrite map_length.
 
-  - subst ty.
-    erewrite map_dtype, map_def_safe_nth. simpl.
+  - rewrite (map_dtype _ (lift #|Γ''| (#|mfix| + #|Γ'|))).
     assert (wf_local Σ (Γ ,,, Γ'' ,,, lift_context #|Γ''| 0 Γ' ,,, lift_context #|Γ''| #|Γ'| (fix_context mfix))).
     subst types.
     apply All_local_env_app in X as [X Hfixc].
     apply All_local_env_app_inv. intuition.
-    revert Hfixc. clear X0 X.
+    revert Hfixc. clear X0 X H.
     induction 1; simpl; auto; try constructor; rewrite lift_context_snoc. econstructor; auto.
     -- destruct t0 as [Ht IHt].
        specialize (IHt Γ (Γ' ,,, Γ0) Γ''). forward IHt.
@@ -1535,6 +862,7 @@ Proof.
        unfold app_context in *. rewrite <- !app_assoc, app_length in IHt.
        specialize (IHt eq_refl). simpl. apply IHt.
     -- eapply type_Fix.
+       rewrite nth_error_map, H. reflexivity.
        now rewrite lift_fix_context.
        rewrite lift_fix_context.
        apply All_map.
@@ -1550,9 +878,7 @@ Proof.
        lia.
        now apply isLambda_lift.
 
-  - subst ty.
-    erewrite map_dtype, map_def_safe_nth. simpl.
-    assert (wf_local Σ (Γ ,,, Γ'' ,,, lift_context #|Γ''| 0 Γ' ,,, lift_context #|Γ''| #|Γ'| (fix_context mfix))).
+  - assert (wf_local Σ (Γ ,,, Γ'' ,,, lift_context #|Γ''| 0 Γ' ,,, lift_context #|Γ''| #|Γ'| (fix_context mfix))).
     subst types.
     apply All_local_env_app in X as [X Hfixc].
     apply All_local_env_app_inv. intuition.
@@ -1581,7 +907,9 @@ Proof.
        rewrite lift_context_app, Nat.add_0_r in IHt.
        unfold app_context in *. rewrite <- !app_assoc, app_length in IHt.
        specialize (IHt eq_refl). simpl. apply IHt.
-    -- eapply type_CoFix.
+    -- rewrite (map_dtype _ (lift #|Γ''| (#|mfix| + #|Γ'|))).
+       eapply type_CoFix.
+       now rewrite nth_error_map, H.
        now rewrite lift_fix_context.
        rewrite lift_fix_context.
        apply All_map.
@@ -1610,26 +938,3 @@ Proof.
   forward t0; eauto.
   forward t0; eauto. now eapply wf_local_app in HΓΓ'.
 Qed.
-
-Inductive subs `{cf : checker_flags} Σ (Γ : context) : list term -> context -> Type :=
-| emptys : subs Σ Γ [] []
-| conss Δ s na t T : subs Σ Γ s Δ ->
-              Σ ;;; Γ |- t : substl s T ->
-              subs Σ Γ (t :: s) (Δ ,, vass na T).
-
-Theorem substitution `{checker_flags} Σ Γ Γ' s Δ (t : term) T :
-  wf Σ -> wf_local Σ Γ ->
-  subs Σ Γ s Γ' ->
-  Σ ;;; Γ ,,, Γ' ,,, Δ |- t : T ->
-  Σ ;;; Γ ,,, map_context (substl s) Δ |- substl s t : substl s T.
-Proof.
-  intros HΣ HΓ * Ht Hu.
-Admitted.
-
-Lemma substitution0 `{checker_flags} Σ Γ n u U (t : term) :
-  wf Σ -> wf_local Σ Γ ->
-  `(Σ ;;; Γ ,, vass n U |- t : T -> Σ ;;; Γ |- u : U ->
-    Σ ;;; Γ |- t {0 := u} : T {0 := u}).
-Proof.
-  intros HΣ HΓ * Ht Hu.
-Admitted.
